Foundation.lean
@@ -73,17 +73,19 @@ import Foundation.Modal.Hilbert.WeakerThan.K4_GL
 import Foundation.Modal.Hilbert.WeakerThan.K4_Grz
 import Foundation.Modal.Hilbert.WeakerThan.K4_K45
 import Foundation.Modal.Hilbert.WeakerThan.K4_S4
-import Foundation.Modal.Hilbert.WeakerThan.K45_KB4
 import Foundation.Modal.Hilbert.WeakerThan.K4_Triv
+import Foundation.Modal.Hilbert.WeakerThan.K45_KB4
 import Foundation.Modal.Hilbert.WeakerThan.K5_K45
+import Foundation.Modal.Hilbert.WeakerThan.KB_KDB
+import Foundation.Modal.Hilbert.WeakerThan.KB5_S5
+import Foundation.Modal.Hilbert.WeakerThan.KD_KDB
 import Foundation.Modal.Hilbert.WeakerThan.KD_KT
 import Foundation.Modal.Hilbert.WeakerThan.KDB_KTB
 import Foundation.Modal.Hilbert.WeakerThan.KT_Grz
 import Foundation.Modal.Hilbert.WeakerThan.KT_KTB
 import Foundation.Modal.Hilbert.WeakerThan.KT_S4
-import Foundation.Modal.Hilbert.WeakerThan.S4_S5
-import Foundation.Modal.Hilbert.WeakerThan.KB5_S5
 import Foundation.Modal.Hilbert.WeakerThan.KTB_S5
+import Foundation.Modal.Hilbert.WeakerThan.S4_S5
 
 import Foundation.Modal.Hilbert.Equiv.GL
 import Foundation.Modal.Hilbert.Equiv.KD_KP
